iris/program_logic/weakestpre.v
@@ -425,9 +425,10 @@ Section proofmode_classes.
   Implicit Types e : expr Λ.
 
   Global Instance frame_wp p s E e R Φ Ψ :
-    (∀ v, Frame p R (Φ v) (Ψ v)) →
+    (class_instances_frame.FrameNoInstantiateExist →
+     ∀ v, Frame p R (Φ v) (Ψ v)) →
     Frame p R (WP e @ s; E {{ Φ }}) (WP e @ s; E {{ Ψ }}) | 2.
-  Proof. rewrite /Frame=> HR. rewrite wp_frame_l. apply wp_mono, HR. Qed.
+  Proof. rewrite /Frame=> HR. rewrite wp_frame_l. apply wp_mono, HR, I. Qed.
 
   Global Instance is_except_0_wp s E e Φ : IsExcept0 (WP e @ s; E {{ Φ }}).
   Proof. by rewrite /IsExcept0 -{2}fupd_wp -except_0_fupd -fupd_intro. Qed.
